BISHOP.dfy
@@ -2,6 +2,51 @@
 include "Ownership-Parallel.dfy"
 include "Context.dfy"
 
+lemma WhyDoesntThisWork(o : Object, pivot : Object, remainder : Owner)
+  requires o.Ready()
+  requires pivot.Ready()
+  requires strictlyInside(o, pivot)
+  requires remainder == (o.AMFO - pivot.AMFO)
+   ensures o.AMFO > pivot.AMFO
+   ensures isFlat(o.AMFO)
+   ensures (o.AMFO - pivot.AMFO) >= (set x <- o.AMFO | x !in pivot.AMFO)
+   ensures (o.AMFO - pivot.AMFO) <= (set x <- o.AMFO | x !in pivot.AMFO)
+   ensures remainder == (set x <- o.AMFO | x !in pivot.AMFO)
+   ensures remainder == (o.AMFO - pivot.AMFO)
+
+
+//   ensures (o.AMFO - pivot.AMFO) >= (set x <- o.AMFO | x.AMFO >= pivot.AMFO)
+ //  ensures (o.AMFO - pivot.AMFO) <= (set x <- o.AMFO | x.AMFO <= pivot.AMFO)
+
+
+
+
+   ensures forall x <- pivot.AMFO :: x in o.AMFO
+   ensures forall x <- pivot.AMFO :: o.AMFO >= pivot.AMFO >= x.AMFO
+
+   ensures forall r <- remainder :: (r in o.AMFO) && (r !in pivot.AMFO)
+
+//   ensures forall r <- remainder :: (r in o.AMFO) && (r !in pivot.AMFO)
+
+   ensures forall r <- remainder :: (r.AMFO > pivot.AMFO)
+
+  ensures forall x <- o.AMFO, p <- pivot.AMFO ::
+
+    ensures forall x <- o.AMFO :: (x in remainder) == (x !in pivot.AMFO)
+   //    ensures remainder == (set x <- o.AMFO | x.AMFO !in pivot.AMFO)
+{}
+
+lemma singel(o : Object)
+  requires o.Ready()
+  // requires AllReady(oo)
+  // requires isFlat(oo)
+  // requires oo > {}n
+  // ensures forall o <- oo, xx <- o.AMFO :: xx in oo
+//   ensures exists x <- oo :: forall y <- oo :: x.AMFO >= y.AMFO
+   ensures exists x <- o.AMFO :: x.AMFO == o.AMFO
+{}
+
+
 
 lemma All_Fucked_Up(obelow : Owner, oabove : Owner, cbelow : Owner, cabove : Owner, m : Klon)
   requires AllReady(obelow)
